Improve automation

Constr/MapLookup.v
@@ -5,81 +5,67 @@ Require Export MapBasics.
 
 Set Implicit Arguments.
 
-Section MapLookup.
-  Open Scope fmap_scope.
-  Variable X : Type.
-  Context `{OrderedType X}.
-  Variable Y : Type.
+Definition lookup_set X `{OrderedType X} Y `{OrderedType Y} (m:X -> Y) (s:set X) : set Y :=
+  SetConstructs.map m s.
 
-  (* Functions are always functional with respect to leibniz equality
-   maps are functional w.r.t. the decidable equality they are parameterized over
-   *)
-
-  Definition lookup_set `{OrderedType Y} (m:X -> Y) (s:set X) : set Y :=
-    SetConstructs.map m s.
-
-  Lemma lookup_set_spec `{OrderedType Y} (m:X -> Y) s y `{Proper _ (_eq ==> _eq) m}
+Lemma lookup_set_spec X `{OrderedType X} Y `{OrderedType Y} (m:X -> Y) s y `{Proper _ (_eq ==> _eq) m}
   : y ∈ lookup_set m s <-> exists x, x ∈ s /\ y === m x.
-  Proof.
-    intros. unfold lookup_set. eapply SetConstructs.map_spec; eauto.
-  Qed.
+Proof.
+  intros. unfold lookup_set. eapply SetConstructs.map_spec; eauto.
+Qed.
 
-  Lemma lookup_set_helper `{OrderedType Y} (m:X -> Y) s x `{Proper _ (_eq ==> _eq) m}
+
+Ltac rewrite_lookup_set dummy := match goal with
+                                | [ H : context [ In ?y (lookup_set ?f ?s) ] |- _ ] =>
+                                  rewrite (@lookup_set_spec _ _ _ _ f s y) in H
+                                | [ |- context [ In ?y (lookup_set ?f ?s) ]] =>
+                                  rewrite (@lookup_set_spec _ _ _ _ f s y)
+                                end.
+Ltac lset_tac := set_tac rewrite_lookup_set.
+
+
+Lemma lookup_set_helper X `{OrderedType X} Y `{OrderedType Y} (m:X -> Y) s x `{Proper _ (_eq ==> _eq) m}
   : x ∈ s -> m x ∈ lookup_set m s.
-  Proof.
-    intros. eapply SetConstructs.map_spec; eauto.
-  Qed.
+Proof.
+  intros. eapply SetConstructs.map_spec; eauto.
+Qed.
 
-  Lemma lookup_set_incl `{OrderedType Y} s t (m:X -> Y) `{Proper _ (_eq ==> _eq) m}
+Lemma lookup_set_incl X `{OrderedType X} Y `{OrderedType Y} s t (m:X -> Y) `{Proper _ (_eq ==> _eq) m}
   : s ⊆ t -> (lookup_set m s) ⊆ (lookup_set m t).
-  Proof.
-    intros P I; hnf. intros Q.
-    eapply lookup_set_spec in Q; [|now eauto].
-    decompose records. eapply lookup_set_spec; eauto.
-  Qed.
+Proof.
+  intros P I; hnf. intros Q.
+  eapply lookup_set_spec in Q; [|now eauto].
+  decompose records. eapply lookup_set_spec; eauto.
+Qed.
 
-  Lemma lookup_set_union `{OrderedType Y} s t (m:X -> Y) `{Proper _ (_eq ==> _eq) m}
+Lemma lookup_set_union X `{OrderedType X} Y `{OrderedType Y} s t (m:X -> Y) `{Proper _ (_eq ==> _eq) m}
   : (lookup_set m (s ∪ t)) [=] (lookup_set m s ∪ lookup_set m t).
-  Proof.
-    intro. split; intros.
-    - eapply lookup_set_spec in H2; eauto.
-      cset_tac.
-      + left. eapply lookup_set_spec; firstorder.
-      + right; eapply lookup_set_spec; firstorder.
-    - cset_tac; eapply lookup_set_spec in H3; dcr; eauto.
-      + eapply lookup_set_spec; eauto. eexists x; cset_tac; firstorder.
-      + eapply lookup_set_spec; eauto. eexists x; cset_tac; firstorder.
-  Qed.
+Proof.
+  intro. split; intros; lset_tac.
+Qed.
 
-  Lemma lookup_set_minus_incl `{OrderedType Y}
-        (s t:set X) (m:X -> Y) `{Proper _ (_eq ==> _eq) m}
+Lemma lookup_set_minus_incl X `{OrderedType X} Y `{OrderedType Y}
+      (s t:set X) (m:X -> Y) `{Proper _ (_eq ==> _eq) m}
   : lookup_set m s \ (lookup_set m t) ⊆ lookup_set m (s \ t).
-  Proof.
-    intros; hnf; intros.
-    edestruct minus_in_in; eauto. eapply lookup_set_spec; eauto.
-    eapply lookup_set_spec in H3; decompose records.
-    eexists x; split; eauto. eapply in_in_minus; eauto.
-    intro. eapply H4. eapply lookup_set_spec. intuition.
-    eexists x; eauto. intuition.
-  Qed.
+Proof.
+  lset_tac.
+  eexists x; split; eauto.
+Qed.
 
-  Lemma lookup_set_minus_single_incl `{OrderedType Y}
-        (s:set X) x (m:X -> Y) `{Proper _ (_eq ==> _eq) m}
+Lemma lookup_set_minus_single_incl X `{OrderedType X} Y `{OrderedType Y}
+      (s:set X) x (m:X -> Y) `{Proper _ (_eq ==> _eq) m}
   : lookup_set m s \ singleton (m x) ⊆ lookup_set m (s \ singleton x).
-  Proof.
-    intros; hnf; intros.
-    eapply lookup_set_minus_incl; eauto.
-  Qed.
-
-End MapLookup.
+Proof.
+  intros; hnf; intros.
+  eapply lookup_set_minus_incl; eauto.
+Qed.
 
 Arguments lookup_set {X} {H} {Y} {H0} m s.
 
 Lemma lookup_set_on_id {X} `{OrderedType X} (s t : set X)
   : s ⊆ t -> (lookup_set (fun x => x) s) ⊆ t.
 Proof.
-  intros. hnf; intros.
-  eapply lookup_set_spec in H1; intuition. firstorder. rewrite H2; auto.
+  lset_tac. rewrite H4; eauto.
 Qed.
 
 
@@ -88,35 +74,30 @@ Global Instance lookup_set_morphism {X} `{OrderedType X} {Y} `{OrderedType Y} {f
   : Proper (Subset ==> Subset) (lookup_set f).
 Proof.
   unfold Proper, respectful, Subset; intros.
-  eapply lookup_set_spec. firstorder. eapply lookup_set_spec in H3.
-  decompose records. eexists x0. split. eauto. rewrite H6. eapply H1.
-  firstorder. eauto.
+  lset_tac.
 Qed.
 
 Global Instance lookup_set_morphism_eq {X} `{OrderedType X} {Y} `{OrderedType Y} {f:X->Y}
  `{Proper _ (_eq ==> _eq) f}
   : Proper (Equal ==> Equal) (lookup_set f).
 Proof.
-  unfold Proper, respectful, Subset; intros. eapply double_inclusion in H2; dcr.
-  split; intros. rewrite <- H3; eauto. rewrite <- H4; eauto.
+  unfold Proper, respectful, Subset; intros ? ? A.
+  eapply double_inclusion in A; dcr. lset_tac.
 Qed.
 
 Lemma lookup_set_singleton {X} `{OrderedType X} {Y} `{OrderedType Y} (f:X->Y)
   `{Proper _ (_eq ==> _eq) f} x
   : lookup_set f {{x}} [=] {{f x}}.
 Proof.
-  cset_tac; intuition.
+  cset_tac.
 Qed.
 
 Lemma lookup_set_singleton' {X} `{OrderedType X} {Y} `{OrderedType Y} (f:X->Y)
   `{Proper _ (_eq ==> _eq) f} x
   : lookup_set f (singleton x) [=] singleton (f x).
 Proof.
-  cset_tac.
-  - eapply lookup_set_spec in H2; dcr; eauto.
-    cset_tac; rewrite H4; eauto.
-  - eapply lookup_set_spec; eauto.
-    eexists x; cset_tac; eauto.
+  lset_tac.
+  - rewrite H4; eauto.
 Qed.
 
 
@@ -126,33 +107,16 @@ Lemma lookup_set_single X `{OrderedType X} Y `{OrderedType Y} (ϱ:X->Y)
   -> lookup_set ϱ D ⊆ D'
   -> {{ ϱ v }} ⊆ D'.
 Proof.
-  intros. hnf; intros.
-  eapply H3. cset_tac; intuition.
-  eapply lookup_set_spec; eauto.
+  intros. lset_tac.
+  eapply H3. lset_tac.
 Qed.
 
 Lemma lookup_set_add X `{OrderedType X} Y `{OrderedType Y} x s (m:X -> Y) `{Proper _ (_eq ==> _eq) m}
 : (lookup_set m {x; s}) [=] {m x; lookup_set m s}.
 Proof.
-  intro. split; intros.
-  - eapply lookup_set_spec in H2; eauto.
-    cset_tac.
-    + left; rewrite H2; symmetry; eauto.
-    + right; eapply lookup_set_spec; firstorder.
-  - cset_tac; eapply lookup_set_spec; eauto.
-    + eexists x; cset_tac; firstorder.
-    + eapply lookup_set_spec in H3; eauto.
-      firstorder.
+  intro. lset_tac.
+  rewrite H2; eauto.
 Qed.
-
-Ltac rewrite_lookup_set dummy := match goal with
-           | [ H : context [ In ?y (lookup_set ?f ?s) ] |- _ ] =>
-             rewrite (@lookup_set_spec _ _ _ _ f s y) in H
-           | [ |- context [ In ?y (lookup_set ?f ?s) ]] =>
-             rewrite (@lookup_set_spec _ _ _ _ f s y)
-           end.
-Ltac lset_tac := set_tac rewrite_lookup_set.
-
 
 Lemma lookup_set_empty X `{OrderedType X} Y `{OrderedType Y} (ϱ:X->Y)
       `{Proper _ (_eq ==> _eq) ϱ}
